spec+proof: change timeArgSize to timeArgLen
Improve the setup of this constant and make it more consistent with
master by renaming timeArgSize to timeArgLen and sharing it between both
the design and abstract specs.

Signed-off-by: Corey Lewis <corey.lewis@proofcraft.systems>

spec/haskell/src/SEL4/Config.lhs
@@ -51,6 +51,6 @@ Also related to interrupt latency, clearing of memory before "Retype" is done on
 > resetChunkBits :: Int
 > resetChunkBits = error "see Kernel_Config.thy"
 
-> timeArgSize :: Int
-> timeArgSize = 64 `div` wordBits
+> timeArgLen :: Int
+> timeArgLen = 64 `div` wordBits
 
