spec/design/skel/Structs_B.thy
@@ -22,4 +22,7 @@ text \<open>Ticks are always 64 bits, even on 32-bit platforms\<close>
 type_synonym ticks_len = 64
 type_synonym ticks = "ticks_len word"
 
+definition timeArgLen :: nat where
+  "timeArgLen \<equiv> LENGTH(ticks_len) div LENGTH(machine_word_len)"
+
 end
